theories/os/refine_ra.v
@@ -4,11 +4,11 @@ From iris_os.os Require Import spec.
 
 Section algebra.
   Context `{K : nat}.
-  
+
   Inductive view : Set := master | snapshot.
 
   Definition max_view (v1 v2: view) :=
-    match v1, v2 with 
+    match v1, v2 with
       | master, _ => master
       | _, master => master
       | _, _ => snapshot
@@ -19,29 +19,29 @@ Section algebra.
 
   Instance comm_max_view: Comm (=) max_view.
   Proof. intros [|] [|]; auto. Qed.
-  
+
   Definition cfg: Type := spec_state * spec_code.
-  
+
   Record refine_car (K': nat) : Type :=
     Refine {
-        refine_view: view; 
+        refine_view: view;
         cfgs: list cfg;
       }.
-  
+
   Arguments refine_view {_} _.
   Arguments cfgs {_} _.
   Arguments Refine {_} _ _.
 
   Definition spec_step' (c c': cfg) : Prop :=
     spec_step (c.2) (c.1) (c'.2) (c'.1).
-  
+
   Inductive valid_cfgs: list cfg → Prop :=
   | VCnil: valid_cfgs []
   | VCsingle c: valid_cfgs [c]
   | VCstep c c' cs:
       spec_step' c c' →
-      valid_cfgs (c' :: cs) →
-      valid_cfgs (c :: c' :: cs).
+      valid_cfgs (c :: cs) →
+      valid_cfgs (c' :: c :: cs).
 
   Global Instance refine_equiv : Equiv (refine_car K) := (=).
 
@@ -52,27 +52,40 @@ Section algebra.
   Proof. by intro. Qed.
 
   Instance refine_valid : Valid (refine_car K) := λ r, valid_cfgs (cfgs r).
-  
+
   Instance refine_core : Core (refine_car K) :=
     λ r, Refine snapshot (cfgs r).
 
-  Inductive refine_disjoint : Disjoint (refine_car K) := 
+  Inductive refine_disjoint : Disjoint (refine_car K) :=
   | snap_snap_disjoint cs1 cs2 :
       (prefix cs1 cs2 ∨ prefix cs2 cs1) →
       Refine snapshot cs1 ⊥ Refine snapshot cs2
   | snap_master_disjoint cs1 cs2:
-      Refine snapshot cs1 ⊥ Refine master (cs1 ++ cs2)
+      Refine snapshot cs1 ⊥ Refine master (cs2 ++ cs1)
   | master_snapshot_disjoint cs1 cs2:
-      Refine master (cs1 ++ cs2) ⊥ Refine snapshot cs1.
+      Refine master (cs2 ++ cs1) ⊥ Refine snapshot cs1.
 
   Existing Instance refine_disjoint.
 
   Instance refine_op : Op (refine_car K) :=
     λ r1 r2,
-    match le_dec (length (cfgs r1)) (length (cfgs r2)) with
-      | left _ => Refine (max_view (refine_view r1) (refine_view r2)) (cfgs r2)
-      | right _ => Refine (max_view (refine_view r1) (refine_view r2)) (cfgs r1)
-    end.
+    if (Nat.leb (length (cfgs r1)) (length (cfgs r2)))
+      then Refine (max_view (refine_view r1) (refine_view r2)) (cfgs r2)
+      else Refine (max_view (refine_view r1) (refine_view r2)) (cfgs r1).
+
+  Lemma refine_op' cs:
+    Refine master cs ⋅ Refine snapshot cs = Refine master cs.
+  Proof.
+    unfold op, refine_op.
+    simpl. by rewrite Nat.leb_refl.
+  Qed.
+
+  Lemma refine_disj' cs:
+    Refine master cs ⊥ Refine snapshot cs.
+  Proof.
+    replace cs with ([] ++ cs) at 1;
+    [ constructor | apply app_nil_l ].
+  Qed.
 
   Lemma refine_dra : DRAMixin (refine_car K).
   Proof.
@@ -80,20 +93,20 @@ Section algebra.
   Admitted.
 
   Canonical Structure refineDR : draT := DRAT (refine_car K) refine_dra.
-  
+
   Instance refine_car_empty : Empty (refine_car K) := Refine snapshot [].
-  
+
   Instance refine_discrete: CMRADiscrete (validityR (refineDR)).
   Proof. apply _. Qed.
-  
+
   Definition refine_cmra := (validity (refineDR)).
 
   Global Instance refine_empty : Empty (refine_cmra) := to_validity (refine_car_empty).
-  
+
   Lemma refine_unit: UCMRAMixin (refine_cmra).
   Admitted.
 
   Canonical Structure refine_ucmra : ucmraT :=
     (UCMRAT refine_cmra (cmra_ofe_mixin _) (cmra_mixin _) refine_unit).
-  
+
 End algebra.
