theories/os/refine_sound.v
@@ -1,0 +1,97 @@
+Require Import logic.
+From iris.base_logic Require Import soundness gen_heap.
+From iris.base_logic Require Export big_op.
+From iris.algebra Require Import dra gmap agree auth frac.
+From iris.base_logic.lib Require Import wsat fancy_updates.
+From iris.base_logic.lib Require Export namespaces invariants.
+From iris.proofmode Require Import tactics.
+From iris_os.os Require Export spec refine_ra refine.
+Set Default Proof Using "Type".
+Import uPred.
+
+
+Section sound.
+  Context `{specG K Σ, clangG Σ} {N: namespace}.
+
+  Inductive simulate: expr → spec_code → Prop :=
+  | SimVal: ∀ v, simulate (Evalue v) (SCdone (Some v))
+  | SimStep:
+      ∀ σ σ' (Σ Σ': spec_state) e c e' c',
+        cstep e σ e' σ' →
+        spec_step_star c Σ c' Σ →
+        simulate e c.
+
+  Local Hint Constructors simulate.
+
+  From iris.program_logic Require Import language adequacy.
+
+  Notation world σ := (wsat ∗ ownE ⊤ ∗ state_interp σ)%I.
+  Notation wptp t := ([∗ list] ef ∈ t, WP ef {{ _, True }})%I.
+
+Lemma wp_step R e1 σ1 e2 σ2 efs Φ :
+  (R ⊢ |==> ▷ R) →
+  prim_step e1 σ1 e2 σ2 efs →
+  world σ1 ∗ R ∗ WP e1 {{ Φ }} ==∗ ▷ |==> ◇ (world σ2 ∗ R ∗ WP e2 {{ Φ }} ∗ wptp efs).
+Proof.
+  rewrite {1}wp_unfold /wp_pre. iIntros (HR Hstep) "[(Hw & HE & Hσ) [HR [H|[_ H]]]]".
+  { iDestruct "H" as (v) "[% _]". apply val_stuck in Hstep; simplify_eq. }
+  rewrite fupd_eq /fupd_def.
+  iMod ("H" $! σ1 with "Hσ [Hw HE]") as ">(Hw & HE & _ & H)"; first by iFrame.
+  iModIntro; iNext.
+  iMod ("H" $! e2 σ2 efs with "[%] [$Hw $HE]") as ">($ & $ & $ & ? & $)"=>//.
+  by iFrame.
+Qed.
+
+  Lemma wptp_step' R e1 t1 t2 σ1 σ2 Φ :
+    (R ⊢ |==> ▷ R) →
+    step (e1 :: t1,σ1) (t2, σ2) →
+    world σ1 ∗ R ∗ WP e1 {{ Φ }} ∗ wptp t1
+    ==∗ ∃ e2 t2', ⌜t2 = e2 :: t2'⌝ ∗ ▷ |==> ◇ (world σ2 ∗ R ∗ WP e2 {{ Φ }} ∗ wptp t2').
+  Proof.
+    iIntros (HR Hstep) "(HW & HR & He & Ht)".
+    destruct Hstep as [e1' σ1' e2' σ2' efs [|? t1'] t2' ?? Hstep]; simplify_eq/=.
+    - iExists e2', (t2' ++ efs); iSplitR; first eauto.
+      rewrite big_sepL_app. iFrame "Ht". iApply wp_step; try iFrame; eauto.
+    - iExists e, (t1' ++ e2' :: t2' ++ efs); iSplitR; first eauto.
+      rewrite !big_sepL_app !big_sepL_cons big_sepL_app.
+      iDestruct "Ht" as "($ & He' & $)"; iFrame "He".
+      iApply wp_step; try iFrame; eauto.
+  Qed.
+
+  Lemma wptp_steps' R n e1 t1 t2 σ1 σ2 Φ :
+    (R ⊢ |==> ▷ R) →
+    nsteps (@step clang_lang) n (e1 :: t1, σ1) (t2, σ2) →
+    world σ1 ∗ R ∗ WP e1 {{ Φ }} ∗ wptp t1 ⊢
+    Nat.iter (S n) (λ P, |==> ▷ P) (∃ e2 t2',
+    ⌜t2 = e2 :: t2'⌝ ∗ world σ2 ∗ R ∗ WP e2 {{ Φ }} ∗ wptp t2').
+  Proof.
+    revert e1 t1 t2 σ1 σ2; simpl; induction n as [|n IH]=> e1 t1 t2 σ1 σ2 /=.
+    { intros HR. inversion_clear 1. iIntros "?". eauto 10. }
+    iIntros (HR Hsteps) "H". inversion_clear Hsteps as [|?? [t1' σ1']].
+    iMod (wptp_step' with "H") as (e1' t1'') "[% H]"; first eauto; simplify_eq. apply H1.
+    iModIntro; iNext; iMod "H" as ">?". iApply IH=>//.
+    subst. done. Qed.
+
+  Lemma foo' s c:
+    (inv N spec_inv ∗ sstate s ∗ scode c) ⊢ |==> ▷ (inv N spec_inv ∗ sstate s ∗ scode c).
+  Proof.
+    iIntros "?". iModIntro.
+    by iNext. Qed.
+
+  Lemma soudness n e1 t1 σ1 t2 σ2 Σ1 c1 Σ2 v2:
+    nsteps step n (e1 :: t1, σ1) (of_val v2 :: t2, σ2) →
+    world σ1 ∗ (inv N spec_inv ∗ sstate Σ1 ∗ scode c1) ∗
+    WP e1 {{ v, scode (SCdone (Some v)) ∗ sstate Σ2 }} ∗ wptp t1 ⊢
+    Nat.iter (S (S n)) (λ P, |==> ▷ P) ⌜simulate (Evalue v2) c1⌝.
+  Proof.
+    intros. rewrite wptp_steps' //; last by apply foo'.
+    rewrite (Nat_iter_S_r (S n)). apply bupd_iter_mono.
+    iDestruct 1 as (e2 t2') "(% & (Hw & HE & _) & (?&?&?) & [H _])"; simplify_eq.
+    iDestruct (wp_value_inv with "H") as "H". rewrite fupd_eq /fupd_def.
+    iMod ("H" with "[Hw HE]") as ">(_ & _ & (?&?))"; first iFrame.
+    iModIntro. iNext.
+    iDestruct (scode_agree with "[~3 ~1]") as "%"; first iFrame.
+    iPureIntro. by subst.
+  Qed.
+
+End sound.
